VsaIris.lean
@@ -68,5 +68,6 @@ import VsaIris.Interp.EnvSpan
 import VsaIris.Interp.EnvGetSpans
 import VsaIris.Interp.EnvGetHit
 import VsaIris.Interp.EnvSetSpans
+import VsaIris.Interp.EnvSetHit
 import VsaIris.Interp.EnvScan
 import VsaIris.Interp.ProofEnvGet
